examples/pseudo_bool/cp_encoding/cp_to_ilp_extensionalScript.sml
@@ -17,21 +17,12 @@ Definition filter_match_def:
 End
 
 (* encodes ftable_i ⇔ X = Ti, provided that LENGTH X = LENGTH Ti *)
-Definition encode_tuple_eq_def:
-  encode_tuple_eq bnd Xts name n =
-    bimply_bits bnd [Pos (INR (Index name n))]
+Definition cencode_tuple_eq_def:
+  cencode_tuple_eq bnd Xts name n =
+    cbimply_var bnd (INR (Index name n))
       ([],
       MAP (λ(X,t). (1i, Pos (INL (Eq X t)))) Xts,
       &LENGTH Xts)
-End
-
-(* The reifications needed for tuple eq on a given row *)
-Definition reify_tuple_eq_def:
-  reify_tuple_eq bnd Xts name n =
-  let
-    eqs = FLAT $ MAP (λ(X,t). encode_full_eq bnd X t) Xts;
-  in
-    eqs ++ encode_tuple_eq bnd Xts name n
 End
 
 Theorem encode_tuple_eq_sem:
@@ -39,10 +30,10 @@ Theorem encode_tuple_eq_sem:
   EVERY (λ(X,t). wb (INL (Eq X t)) ⇔ varc wi X = t) Xts
   ⇒
   (EVERY (λx. iconstraint_sem x (wi,wb))
-    (encode_tuple_eq bnd Xts name n) ⇔
+    (abstr (cencode_tuple_eq bnd Xts name n)) ⇔
   (wb (INR (Index name n)) ⇔ EVERY (λ(X,t). varc wi X = t) Xts))
 Proof
-  rw[encode_tuple_eq_def,iconstraint_sem_def]>>
+  rw[cencode_tuple_eq_def,iconstraint_sem_def]>>
   simp[eval_lin_term_def]>>
   qho_match_abbrev_tac ‘((P ⇔ R) ⇔ (R ⇔ Q))’>>
   qsuff_tac ‘P ⇔ Q’
@@ -63,10 +54,19 @@ Proof
   intLib.ARITH_TAC
 QED
 
-Definition table_al1_def[simp]:
-  table_al1 Xtss name =
-    (([],
-      MAPi (λn Xts. (1i, Pos (INR (Index name n)))) Xtss, 1):'a aiconstraint)
+(* The reifications needed for tuple eq on a given row *)
+Definition reify_tuple_eq_def:
+  reify_tuple_eq bnd Xts name n =
+  let
+    eqs = FLAT $ MAP (λ(X,t). encode_full_eq bnd X t) Xts;
+  in
+    eqs ++ abstr (cencode_tuple_eq bnd Xts name n)
+End
+
+Definition ctable_al1_def[simp]:
+  ctable_al1 Xtss name =
+     cat_least_one name
+      (MAPi (λn Xts. (Pos (INR (Index name n)))) Xtss)
 End
 
 Definition encode_table_def:
@@ -76,7 +76,7 @@ Definition encode_table_def:
     then
       let Xtss = MAP (λts. filter_match (ZIP (Xs,ts))) tss in
       (FLAT $ MAPi (λn Xts. reify_tuple_eq bnd Xts name n) Xtss) ++
-      [table_al1 Xtss name]
+      abstr (ctable_al1 Xtss name)
     else
       [false_constr]
 End
@@ -99,9 +99,9 @@ Theorem encode_tuple_eq_sem_reify:
   n < LENGTH tss ∧
   LENGTH (EL n tss) = LENGTH Xs ∧
   Xts = filter_match (ZIP (Xs,EL n tss)) ⇒
-  EVERY (λx. iconstraint_sem x (wi,reify_avar cs wi)) (encode_tuple_eq bnd Xts name n)
+  EVERY (λx. iconstraint_sem x (wi,reify_avar cs wi)) (abstr (cencode_tuple_eq bnd Xts name n))
 Proof
-  rw[encode_tuple_eq_def,reify_avar_def,reify_flag_def]>>
+  rw[cencode_tuple_eq_def,reify_avar_def,reify_flag_def]>>
   simp[iconstraint_sem_def,eval_lin_term_def,iterateTheory.LAMBDA_PAIR,
     reify_avar_def,reify_reif_def,MAP_MAP_o,o_DEF,
     match_row_filter_match,EVERY_MEM]
@@ -141,11 +141,9 @@ Proof
     fs[EVERY_MEM]>>metis_tac[MEM_EL])>>
   fs[EVERY_MEM]>>first_x_assum drule>>
   strip_tac>>
-  simp[iconstraint_sem_def,eval_lin_term_def,reify_avar_def,reify_flag_def,
-    o_DEF,miscTheory.MAPi_enumerate_MAP,MAP_MAP_o,iterateTheory.LAMBDA_PAIR]>>
+  simp[MEM_MAPi,PULL_EXISTS,reify_avar_def,reify_flag_def]>>
   qpat_x_assum`MEM _ _` mp_tac>>
   simp[Once MEM_EL]>>rw[]>>
-  simp[EXISTS_PROD]>>
   qexists_tac`n`>>
   simp[MEM_enumerate]
 QED
@@ -197,12 +195,8 @@ Proof
   simp[encode_table_def,table_sem_def]>>
   IF_CASES_TAC>>fs[]>>
   rw[]>>
-  pop_assum mp_tac>>
-  simp[iconstraint_sem_def,eval_lin_term_def,reify_avar_def,reify_flag_def,
-    o_DEF,miscTheory.MAPi_enumerate_MAP,MAP_MAP_o,iterateTheory.LAMBDA_PAIR]>>
-  simp[EXISTS_PROD]>>rw[]>>
-  dxrule MEM_enumerate_0>>
-  rw[]>>
+  gvs[MEM_MAPi]>>
+  qexists_tac`EL n tss`>>
   simp[MEM_EL,PULL_EXISTS]>>
   first_assum $ irule_at Any>>
   DEP_REWRITE_TAC [match_row_filter_match]>>
@@ -245,21 +239,10 @@ Proof
 QED
 
 (* The reifications needed for tuple eq on a given row *)
-
 Definition cencode_full_eqs_def:
   cencode_full_eqs bnd xs ec =
     fold_cenc
       (λXt ec. cencode_full_eq bnd (FST Xt) (SND Xt) ec) xs ec
-End
-
-Definition cencode_tuple_eq_def:
-  cencode_tuple_eq bnd Xts name n =
-    let nm = format_flag (Index name n) in
-    mk_annotate [
-      nm ^ strlit"[f]";
-      nm ^ strlit"[r]"
-    ]
-    (encode_tuple_eq bnd Xts name n)
 End
 
 Definition creify_tuple_eq_def:
@@ -268,19 +251,13 @@ Definition creify_tuple_eq_def:
     (eqs,ec') = cencode_full_eqs bnd Xts ec;
   in
     (Append eqs
-      (List (cencode_tuple_eq bnd Xts name n)), ec')
+      (cencode_tuple_eq bnd Xts name n), ec')
 End
 
 Definition creify_tuple_eqs_def:
   creify_tuple_eqs bnd name nXtss ec =
   fold_cenc
     (λ(n,Xts) ec. creify_tuple_eq bnd Xts name n ec) nXtss ec
-End
-
-Definition ctable_al1_def[simp]:
-  ctable_al1 Xtss name =
-    (SOME (strlit"c[" ^ name ^ strlit"][al1]"),
-      table_al1 Xtss name)
 End
 
 Definition cencode_table_def:
@@ -291,10 +268,9 @@ Definition cencode_table_def:
       let Xtss = MAP (λts. filter_match (ZIP (Xs,ts))) tss in
       let nXtss = enumerate 0 Xtss in
       let (ys,ec') = creify_tuple_eqs bnd name nXtss ec in
-      (Append ys
-        (List [ctable_al1 Xtss name]), ec')
+      (Append ys (ctable_al1 Xtss name), ec')
     else
-      (List [cfalse_constr], ec)
+      (cfalse_constr, ec)
 End
 
 Definition cencode_extensional_constr_def:
@@ -311,10 +287,9 @@ Proof
   rw[cencode_extensional_constr_def,encode_extensional_constr_def]>>
   gvs[CaseEq"extensional_constr"]>>
   fs[encode_table_def,cencode_table_def]>>
-  rw[]>>
-  gvs[UNCURRY_EQ]>>
+  rw[]>>gvs[UNCURRY_EQ]>>
   irule enc_rel_Append>>
-  irule_at Any enc_rel_List_refl_1>>
+  irule_at Any enc_rel_abstr>>
   simp[MAPi_enumerate_MAP]>>
   irule_at Any enc_rel_fold_cenc>>
   fs[creify_tuple_eqs_def]>>
@@ -324,9 +299,7 @@ Proof
   gvs[creify_tuple_eq_def,reify_tuple_eq_def]>>
   pairarg_tac>>gvs[]>>
   irule enc_rel_Append>>
-  simp[cencode_tuple_eq_def]>>
-  irule_at Any enc_rel_List_mk_annotate>>
-  simp[MAPi_enumerate_MAP]>>
+  irule_at Any enc_rel_abstr>>
   irule_at Any enc_rel_fold_cenc>>
   fs[cencode_full_eqs_def]>>
   first_x_assum (irule_at Any)>>
